update _coqproj, makefile and examples

coq/theories/Lib.v
@@ -1,412 +1,430 @@
-
-(* Require Import FStar.Mul. *)
-
 (*** Integers *)
-From Coq Require Import ZArith Vector.
-(* Require Import Int.PArray. *)
-(* From Coq Require Import Numbers.Cyclic.Abstract.CyclicAxioms. *)
-From compcert Require Import Integers.
+From Coq Require Import ZArith List Vector.
+Import ListNotations.
+(* Require Import IntTypes. *)
 
-Require Import IntTypes.
+Require Import MachineIntegers.
+From Coqprime Require GZnZ.
+
+Axiom secret : forall {WS : WORDSIZE},  (@int WS) -> (@int WS). 
 
 
-Definition uint_size := nat.
-(* Definition uint_size := range_t U32. *)
-Definition int_size := nat.
-(* Definition int_size := range_t S32. *)
+(* CompCert integers' signedness is only interpreted through 'signed' and 'unsigned',
+   and not in the representation. Therefore, uints are just names for their respective ints.
+*)
+Definition uint8 := int8.
+Definition uint16 := int16.
+Definition uint32 := int32.
+Definition uint64 := int64.
+Definition uint128 := int128.
 
-Open Scope N_scope.
-(* Definition usize (n:range_t U32) : u:uint_size{u == n} := n *)
-(* Definition isize (n:range_t S32) : u:int_size{u == n} := n *)
+Definition uint_size := int32.
+Definition int_size := int32.
 
-Definition usize {A} (n : A) := id n.
-Definition isize {A} (n : A) := id n.
+(* Represents any type that can be converted to uint_size and back *)
+Class UInt_sizable (A : Type) := {
+  usize : A -> uint_size;
+  from_uint_size : uint_size -> A; 
+}.
+Arguments usize {_} {_}.
+Arguments from_uint_size {_} {_}.
 
-Coercion N.to_nat : N >-> nat. 
-Coercion N.of_nat : nat >-> N. 
-Coercion Z.to_nat : Z >-> nat.
+Global Instance nat_uint_sizable : UInt_sizable nat := {
+  usize n := repr (Z.of_nat n);
+  from_uint_size n := Z.to_nat (unsigned n);
+}.
 
-(* Notation "'usize' n" := (id n) (at level 56) : hacspec_scope. *)
-(* Notation "'isize' n" := (id n) (at level 56) : hacspec_scope. *)
+Global Instance N_uint_sizable : UInt_sizable N := {
+  usize n := repr (Z.of_N n);
+  from_uint_size n := Z.to_N (unsigned n);
+}.
 
-Axiom 
-  uint8
-  uint16
-  uint32
-  uint64
-  uint128
-  int8
-  int16
-  int32
-  int64
-  int128 
-  pub_uint8 
-  pub_int8 
-  pub_uint16 
-  pub_int16 
-  pub_uint32 
-  pub_int32 
-  pub_uint64 
-  pub_int64 
-  pub_uint128 
-  pub_int128 
-  : Type.
+Global Instance Z_uint_sizable : UInt_sizable Z := {
+  usize n := repr n;
+  from_uint_size n := unsigned n;
+}.
 
-(* Definition size_t := uint_t U32 PUB *)
-(* Axiom uint_size : forall (n : inttype), n < U32. *)
-(* Axiom size : (n:size_nat) : size_t = uint #U32 #PUB n *)
 
+(* Same, but for int_size *)
+Class Int_sizable (A : Type) := {
+  isize : A -> int_size;
+  from_int_size : int_size -> A; 
+}.
+
+Arguments isize {_} {_}.
+Arguments from_int_size {_} {_}.
+
+Global Instance nat_Int_sizable : Int_sizable nat := {
+  isize n := repr (Z.of_nat n);
+  from_int_size n := Z.to_nat (signed n);
+}.
+
+Global Instance N_Int_sizable : Int_sizable N := {
+  isize n := repr (Z.of_N n);
+  from_int_size n := Z.to_N (signed n);
+}.
+
+Global Instance Z_Int_sizable : Int_sizable Z := {
+  isize n := repr n;
+  from_int_size n := signed n;
+}.
 
 
 (**** Public integers *)
 
 (* Definition pub_u8 (n:range_t U8) : u:pub_uint8{v u == n} := uint #U8 #PUB n *)
-Definition pub_u8 (n : N) := n.
+Definition pub_u8 (n : Z) : int8 := repr n.
 
 (* Definition pub_i8 (n:N) : u:pub_int8{v u == n} := sint #S8 #PUB n *)
-Definition pub_i8 (n : N) := n.
+Definition pub_i8 (n : Z) : int8 := repr n.
 
 (* Definition pub_u16 (n:N) : u:pub_uint16{v u == n} := uint #U16 #PUB n *)
-Definition pub_u16 (n : N) := n.
+Definition pub_u16 (n : Z) : int16 := repr n.
 
 (* Definition pub_i16 (n:N) : u:pub_int16{v u == n} := sint #S16 #PUB n *)
-Definition pub_i16 (n : N) := n.
+Definition pub_i16 (n : Z) : int16 := repr n.
 
 (* Definition pub_u32 (n:N) : u:pub_uint32{v u == n} := uint #U32 #PUB n *)
-Definition pub_u32 (n : N) := n.
+Definition pub_u32 (n : Z) : int32 := repr n.
 
 (* Definition pub_i32 (n:N) : u:pub_int32{v u == n} := sint #S32 #PUB n *)
-Definition pub_i32 (n : N) := n.
+Definition pub_i32 (n : Z) : int32 := repr n.
 
 (* Definition pub_u64 (n:N) : u:pub_uint64{v u == n} := uint #U64 #PUB n *)
-Definition pub_u64 (n : N) := n.
+Definition pub_u64 (n : Z) : int64 := repr n.
 
 (* Definition pub_i64 (n:N) : u:pub_int64{v u == n} := sint #S64 #PUB n *)
-Definition pub_i64 (n : N) := n.
+Definition pub_i64 (n : Z) : int64 := repr n.
 
 (* Definition pub_u128 (n:N) : u:pub_uint128{v u == n} := uint #U128 #PUB n *)
-Definition pub_u128 (n : N) := n.
+Definition pub_u128 (n : Z) : int128 := repr n.
 
 (* Definition pub_i128 (n:N) : u:pub_int128{v u == n} := sint #S128 #PUB n *)
-Definition pub_i128 (n : N) := n.
+Definition pub_i128 (n : Z) : int128 := repr n.
 
 (**** Operations *)
 
-Axiom size_t : Type.
-Axiom size : forall {intt : Type}, intt -> size_t.
-(* second argument is size *)
-Axiom rotate_left : forall {inttype : Type}, inttype -> size_t -> inttype.
-Axiom rotate_right : forall {inttype : Type}, inttype -> size_t -> inttype.
-Axiom shift_left : forall {inttype shiftval : Type}, inttype -> shiftval -> inttype.
-Axiom shift_right : forall {inttype shiftval : Type}, inttype -> shiftval -> inttype.
+(* Should maybe use size of s instead? *)
+Definition uint8_rotate_left (u: int8) (s: int8) : int8 := rol u s.
 
-Definition uint8_rotate_left (u: uint8) (s: uint8) : uint8 :=
-  rotate_left u (size s).
+Definition uint8_rotate_right (u: int8) (s: int8) : int8 := ror u s.
 
-Definition uint8_rotate_right (u: uint8) (s: uint8) : uint8 :=
-  rotate_right u (size s).
+Definition uint16_rotate_left (u: int16) (s: int16) : int16 :=
+  rol u s.
 
-Definition uint16_rotate_left (u: uint16) (s: uint16) : uint16 :=
-  rotate_left u (size s).
+Definition uint16_rotate_right (u: int16) (s: int16) : int16 :=
+  ror u s.
 
-Definition uint16_rotate_right (u: uint16) (s: uint16) : uint16 :=
-  rotate_right u (size s).
+Definition uint32_rotate_left (u: int32) (s: int32) : int32 :=
+  rol u s.
 
-Definition uint32_rotate_left (u: uint32) (s: uint32) : uint32 :=
-  rotate_left u (size s).
+Definition uint32_rotate_right (u: int32) (s: int32) : int32 :=
+  ror u s.
 
-Definition uint32_rotate_right (u: uint32) (s: uint32) : uint32 :=
-  rotate_right u (size s).
+Definition uint64_rotate_left (u: int64) (s: int64) : int64 :=
+  rol u s.
 
-Definition uint64_rotate_left (u: uint64) (s: uint64) : uint64 :=
-  rotate_left u (size s).
+Definition uint64_rotate_right (u: int64) (s: int64) : int64 :=
+  ror u s.
 
-Definition uint64_rotate_right (u: uint64) (s: uint64) : uint64 :=
-  rotate_right u (size s).
+Definition uint128_rotate_left (u: int128) (s: int128) : int128 :=
+  rol u s.
 
-Definition uint128_rotate_left (u: uint128) (s: uint128) : uint128 :=
-  rotate_left u (size s).
+Definition uint128_rotate_right (u: int128) (s: int128) : int128 :=
+  ror u s.
 
-Definition uint128_rotate_right (u: uint128) (s: uint128) : uint128 :=
-  rotate_right u (size s).
+(* should use size u instead of u? *)
+Definition usize_shift_right (u: uint_size) (s: int32) : uint_size :=
+  (ror u s).
 
-Axiom to_uint_size : size_t -> uint_size.
+(* should use size u instead of u? *)
+Definition usize_shift_left (u: uint_size) (s: int32) : uint_size :=
+  (rol u s).
 
-Definition usize_shift_right (u: uint_size) (s: pub_uint32) : uint_size :=
-  to_uint_size (shift_right (size u) s).
-
-Definition usize_shift_left (u: uint_size) (s: pub_uint32) : uint_size :=
-  to_uint_size (shift_left (size u) s).
+Definition pub_uint128_wrapping_add (x y: int128) : int128 :=
+  add x y.
 
 
-Axiom pub_uint128_wrapping_add : pub_uint128 -> pub_uint128 -> pub_uint128. 
-  (* x +. y *)
+Infix "%%" := Z.rem (at level 40, left associativity) : Z_scope.
+Infix ".+" := (MachineIntegers.add) (at level 77) : hacspec_scope.
+Infix ".-" := (MachineIntegers.sub) (at level 77) : hacspec_scope.
+Infix "./" := (MachineIntegers.divs) (at level 77) : hacspec_scope.
+Infix ".%" := (MachineIntegers.mods) (at level 77) : hacspec_scope.
+Infix ".^" := (MachineIntegers.xor) (at level 77) : hacspec_scope.
+Infix ".&" := (MachineIntegers.and) (at level 77) : hacspec_scope.
+Infix ".|" := (MachineIntegers.or) (at level 77) : hacspec_scope.
+Infix "==" := (MachineIntegers.eq) (at level 32) : hacspec_scope.
+(* Definition one := (@one WORDSIZE32). *)
+(* Definition zero := (@zero WORDSIZE32). *)
 
 (*** Loops *)
 
-Axiom foldi :
-  forall {acc: Type},
-  uint_size ->
-  uint_size ->
-  (uint_size -> acc -> acc) ->
-  acc -> acc.
+(* 
+Fixpoint foldi_
+  {acc: Type}
+  (cur_i: uint_size)
+  (hi: uint_size) (* {cur_i <= hi} *)
+  (f: uint_size -> acc -> acc) (* {i < hi} *)
+  (cur: acc)
+    : acc :=
 
-(*** Sequences (lists) *)
-From Coq Require Import List.
+  if cur_i == hi then cur else
+  foldi_ (cur_i + one) hi f (f cur_i cur). *)
 
-(* module LSeq := Lib.Sequence *)
-(* module LBSeq := Lib.ByteSequence *)
+Open Scope nat_scope.
+Fixpoint foldi_ 
+  {acc : Type}
+  (fuel : nat)
+  (i : uint_size)
+  (f : uint_size -> acc -> acc)
+  (cur : acc) : acc :=
+  match fuel with
+  | 0 => cur
+  | S n' => foldi_ n' (add i one) f (f i cur)
+  end.
+Close Scope nat_scope.
+Definition foldi
+  {acc: Type}
+  (lo: uint_size)
+  (hi: uint_size) (* {lo <= hi} *)
+  (f: (uint_size) -> acc -> acc) (* {i < hi} *)
+  (init: acc) : acc :=
+  match Z.sub (unsigned hi) (unsigned lo) with
+  | Z0 => init
+  | Zneg p => init
+  | Zpos p => foldi_ (Pos.to_nat p) lo f init
+  end.
 
-(* We use vectors to define lseq *)
-Definition lseq := Vector.t.
+(* Coercion Int32.repr : Z >-> int. *)
+(* Definition N_to_int n : int := Z.of_N n. *)
+(* Coercion N_to_int : N >-> int. *)
 
-(* Definition lseq_to_list {A len} (s : lseq A len) := 
-  match s with
-  | mkLseq _ _ l => l
-  end. *)
+(* Compute (foldi 1 2 (fun i acc => i + 1) 0). *)
 
-(* simplification *)
+(*** Seq *)
+
+(* module LSeq = Lib.Sequence *)
+(* module LBSeq = Lib.ByteSequence *)
+
+
+Definition nseq := Vector.t.
+(* Definition lseq (A : Type) (len : uint_size) := Vector.t A (from_uint_size len). *)
+
 Definition seq (A : Type) := list A.
 
+(* Automatic conversion from nseq/vector/array to seq/list *)
+Global Coercion Vector.to_list : Vector.t >-> list.
+
+Definition byte_seq := seq int8.
 Definition list_len := length.
 
-Definition byte_seq := seq uint8.
-
-Definition nseq (A : Type) (len: nat) := lseq A len.
 
 Definition seq_len {A: Type} (s: seq A) : N := N.of_nat (length s).
 
-Definition seq_new_ {A: Type} (init : A) (len: uint_size) : lseq A len :=
+
+
+Definition seq_new_ {A: Type} (init : A) (len: nat) : nseq A len :=
   const init len.
 
-Definition array_from_list {A: Type} (l: list A) : lseq A (length l)
+(* Fixpoint of_list {A} (l : list A) : lseq A (usize (length l)) :=
+match l as l' return lseq A (usize (length l')) with
+  |Datatypes.nil => Vector.nil _
+  |(h :: tail)%list => (Vector.cons _ h (usize (1 + length l)) (of_list tail))
+end. *)
+
+Definition array_from_list (A: Type) (l: list A) : nseq A (length l)
   := of_list l.
+
+(* automatic conversion from list to array *)
+Global Coercion array_from_list : list >-> nseq.
 
 (**** Array manipulation *)
 
-Axiom array_default_val : forall A, A.
+Class Default (A : Type) := {
+  default : A
+}.
 
-Definition array_new_ {A: Type} (init:A) (len: uint_size)  : lseq A len :=
+(* Default instances for common types *)
+Global Instance nat_default : Default nat := {
+  default := 0%nat
+}.
+Global Instance N_default : Default N := {
+  default := 0%N
+}.
+Global Instance Z_default : Default Z := {
+  default := 0%Z
+}.
+Global Instance uint_size_default : Default uint_size := {
+  default := zero
+}.
+Global Instance int_size_default : Default int_size := {
+  default := zero
+}.
+Global Instance int_default {WS : WORDSIZE} : Default int := {
+  default := repr 0
+}.
+Global Arguments default {_} {_}.
+
+
+Definition array_new_ {A: Type} (init:A) (len: nat)  : nseq A len :=
   const init len.
 
-Check (Fin.t 4).
 Open Scope nat_scope.
-Definition array_index {A: Type} {len : uint_size} (s: lseq A len) (i: uint_size) {H : i < len} : A :=
-  Vector.nth s (Fin.of_nat_lt H). 
+Definition array_index {A: Type} `{Default A} {len : nat} (s: nseq A len) (i: nat) : A.
+Proof.
+  destruct (i <? len) eqn:H1.
+  (* If i < len, index normally *)
+  - rewrite Nat.ltb_lt in H1. 
+    exact (Vector.nth s (Fin.of_nat_lt H1)). 
+  (* otherwise return default element *)
+  - exact default.
+Defined.
 
-  (* Definition array_index {A: Type} {len : uint_size} (s: lseq A len) (i: uint_size) : A :=
-  List.nth (N.to_nat i) (lseq_to_list s). *)
 
-Definition array_upd {A: Type} {len : uint_size} (s: lseq A len) (i: uint_size) (new_v: A) {H : i < len} : lseq A len :=
-  Vector.replace s (Fin.of_nat_lt H) new_v.
+Definition array_upd {A: Type} {len : nat} (s: nseq A len) (i: nat) (new_v: A) : nseq A len.
+Proof.
+  destruct (i <? len) eqn:H.
+  (* If i < len, update normally *)
+  - rewrite Nat.ltb_lt in H. 
+    exact (Vector.replace s (Fin.of_nat_lt H) new_v).
+  (* otherwise return original array *)
+  - exact s.
+Defined.
 
 (* Definition array_upd {A: Type} {len : uint_size} (s: lseq A len) (i: uint_size) (new_v: A) : lseq A len := List.upd s i new_v. *)
 
 Definition array_from_seq
   {a: Type}
-  (out_len:uint_size)
+  (out_len:nat)
   (input: seq a)
   (* {H : List.length input = out_len} *)
     : t a (length input) :=
   Vector.of_list input.
 
 Definition slice {A} (l : seq A) (i j : nat) : seq A := 
-  if j <=? i then nil else firstn (j-i+1) (skipn i l).
-Import ListNotations.
+  if j <=? i then [] else firstn (j-i+1) (skipn i l).
 
 (* Compute (slice [1;2;3;4;5] 1 0). *)
+
+Definition lseq_slice {A n} (l : nseq A n) (i j : nat) : nseq A _ :=
+  of_list (slice (to_list l) i j).
+
+
 (* 
+
 Definition update_sub {A len slen} (v : t A len) (i n) (sub : t A slen) :=
   Vector.append
     (Vector.append (slice v 0 start ) sub) *)
 
+Axiom update_sub : forall {A len slen}, t A len -> nat -> nat -> seq A -> t A slen.
 
-(* Definition array_from_slice
+Definition array_from_slice
   {a: Type}
   (default_value: a)
-  (out_len: uint_size)
+  (out_len: nat)
   (input: seq a)
-  (start: uint_size)
-  (*   (slice_len: uint_size{start + slice_len <= LSeq.length input /\ slice_len <= out_len}) *)
-  (slice_len: uint_size)
-    : lseq a out_len :=
-    let out := Vector.const out_len default_value in
-    LSeq.update_sub out 0 slice_len (LSeq.slice  input start (start + slice_len)). Admitted.
-   *)
+  (start: nat)
+  (slice_len: nat)
+    : nseq a out_len :=
+    let out := const default_value out_len in
+    update_sub out 0 slice_len (slice input start (start + slice_len)).
+  
 
 Definition array_slice
   {a: Type}
   (input: seq a)
-  (start: uint_size)
-  (slice_len: uint_size)
-    : lseq a slice_len.
-  Admitted.
+  (start: nat)
+  (slice_len: nat)
+    : nseq a _ :=
+  let out := slice input start (start + slice_len) in
+  array_from_seq slice_len out.
+
 
 Definition array_from_slice_range
   {a: Type}
   (default_value: a)
-  (out_len: uint_size)
+  (out_len: nat)
   (input: seq a)
   (start_fin: (uint_size * uint_size))
-    : lseq a out_len. Admitted.
-    
+    : nseq a out_len :=
+    let out := array_new_ default_value out_len in
+    let (start, fin) := start_fin in
+    update_sub out 0 ((from_uint_size fin) - (from_uint_size start)) (slice input (from_uint_size start) (from_uint_size fin)).
+
+  
 Definition array_slice_range
   {a: Type}
-  {len : uint_size}
-  (input: lseq a len)
+  {len : nat}
+  (input: nseq a len)
   (start_fin:(uint_size * uint_size))
-    : lseq a (snd start_fin - fst start_fin). Admitted.
+    : nseq a _ :=
+  lseq_slice input (from_uint_size (fst start_fin)) (from_uint_size (snd start_fin)).
+  
 
 Definition array_update_start
   {a: Type}
-  {len: uint_size}
-  (s: lseq a len)
+  {len: nat}
+  (s: nseq a len)
   (start_s: seq a)
-    : lseq a len. Admitted.
+    : nseq a len :=
+    update_sub s 0 (length start_s) start_s.
 
-Definition array_len  {a: Type} {len: uint_size} (s: lseq a len) := len.
+
+Definition array_len  {a: Type} {len: nat} (s: nseq a len) := len.
 
 (**** Seq manipulation *)
 
 Definition seq_slice
   {a: Type}
   (s: seq a)
-  (start: uint_size)
-  (len: uint_size)
-    : lseq a len. Admitted.
+  (start: nat)
+  (len: nat)
+    : nseq a _ :=
+  array_from_seq len (slice s start (start + len)).
+
 
 Definition seq_update
-  {a: Type}Definition nseq (A : Type) (len: nat) := lseq A len.
-
-  Definition seq_len {A: Type} (s: seq A) : N := N.of_nat (length s).
-  
-  Definition seq_new_ {A: Type} (init : A) (len: uint_size) : lseq A len :=
-    const init len.
-  
-  Definition array_from_list {A: Type} (l: list A) : lseq A (length l)
-    := of_list l.
-  
-  (**** Array manipulation *)
-  
-  Axiom array_default_val : forall A, A.
-  
-  Definition array_new_ {A: Type} (init:A) (len: uint_size)  : lseq A len :=
-    const init len.
-  
-  Check (Fin.t 4).
-  Open Scope nat_scope.
-  Definition array_index {A: Type} {len : uint_size} (s: lseq A len) (i: uint_size) {H : i < len} : A :=
-    Vector.nth s (Fin.of_nat_lt H). 
-  
-    (* Definition array_index {A: Type} {len : uint_size} (s: lseq A len) (i: uint_size) : A :=
-    List.nth (N.to_nat i) (lseq_to_list s). *)
-  
-  Definition array_upd {A: Type} {len : uint_size} (s: lseq A len) (i: uint_size) (new_v: A) {H : i < len} : lseq A len :=
-    Vector.replace s (Fin.of_nat_lt H) new_v.
-  
-  (* Definition array_upd {A: Type} {len : uint_size} (s: lseq A len) (i: uint_size) (new_v: A) : lseq A len := List.upd s i new_v. *)
-  
-  Definition array_from_seq
-    {a: Type}
-    (out_len:uint_size)
-    (input: seq a)
-    (* {H : List.length input = out_len} *)
-      : t a (length input) :=
-    Vector.of_list input.
-  
-  Definition slice {A} (l : seq A) (i j : nat) : seq A := 
-    if j <=? i then nil else firstn (j-i+1) (skipn i l).
-  Import ListNotations.
-  
-  (* Compute (slice [1;2;3;4;5] 1 0). *)
-  (* 
-  Definition update_sub {A len slen} (v : t A len) (i n) (sub : t A slen) :=
-    Vector.append
-      (Vector.append (slice v 0 start ) sub) *)
-  
-  
-  (* Definition array_from_slice
-    {a: Type}
-    (default_value: a)
-    (out_len: uint_size)
-    (input: seq a)
-    (start: uint_size)
-    (*   (slice_len: uint_size{start + slice_len <= LSeq.length input /\ slice_len <= out_len}) *)
-    (slice_len: uint_size)
-      : lseq a out_len :=
-      let out := Vector.const out_len default_value in
-      LSeq.update_sub out 0 slice_len (LSeq.slice  input start (start + slice_len)). Admitted.
-     *)
-  
-  Definition array_slice
-    {a: Type}
-    (input: seq a)
-    (start: uint_size)
-    (slice_len: uint_size)
-      : lseq a slice_len.
-    Admitted.
-  
-  Definition array_from_slice_range
-    {a: Type}
-    (default_value: a)
-    (out_len: uint_size)
-    (input: seq a)
-    (start_fin: (uint_size * uint_size))
-      : lseq a out_len. Admitted.
-      
-  Definition array_slice_range
-    {a: Type}
-    {len : uint_size}
-    (input: lseq a len)
-    (start_fin:(uint_size * uint_size))
-      : lseq a (snd start_fin - fst start_fin). Admitted.
-  
-  Definition array_update_start
-    {a: Type}
-    {len: uint_size}
-    (s: lseq a len)
-    (start_s: seq a)
-      : lseq a len. Admitted.
-  
-  Definition array_len  {a: Type} {len: uint_size} (s: lseq a len) := len.
-  
-  (**** Seq manipulation *)
-  
-  Definition seq_slice
-    {a: Type}
-    (s: seq a)
-    (start: uint_size)
-    (len: uint_size)
-      : lseq a len. Admitted.
-  
-  Definition seq_update
-    {a: Type}
-    (s: seq a)
-    (start: uint_size)
-    (input: seq a)
+  {a: Type}
   (s: seq a)
-  (start: uint_size)
+  (start: nat)
   (input: seq a)
-    : nseq a (length s). Admitted.
+    : nseq a (length s) :=
+  update_sub (of_list s) start (length input) input.
+
+Definition sub {a} (s : list a) start n := 
+  slice s start (start + n).
+
+Definition seq_update_slice
+  {a : Type}
+  (out: seq a)
+  (start_out: nat)
+  (input: seq a)
+  (start_in: nat)
+  (len: nat)
+    : nseq a (length out)
+  :=
+  update_sub (of_list out) start_out len
+    (sub input start_in len).
 
 Definition seq_concat
-  {a: Type}
+  {a : Type}
   (s1 :seq a)
   (s2: seq a)
-  : lseq a (length s1 + length s2).
-  Admitted.
+  : nseq a _ :=
+  of_list (List.rev_append s1 s2).
+
 
 (**** Chunking *)
 
-Definition seq_num_chunks {a: Type} (s: seq a) (chunk_len: uint_size) : uint_size :=
+Definition seq_num_chunks {a: Type} (s: seq a) (chunk_len: nat) : nat :=
   ((length s) + chunk_len - 1) / chunk_len. 
 
 Definition seq_chunk_len
   {a: Type}
   (s: seq a)
-  (chunk_len: uint_size)
-  (chunk_num: uint_size)
-    : uint_size :=
+  (chunk_len: nat)
+  (chunk_num: nat)
+    : nat :=
   let idx_start := chunk_len * chunk_num in
   if (length s) <? idx_start + chunk_len then
     (length s) - idx_start
@@ -416,404 +434,493 @@ Definition seq_chunk_len
 (* Definition seq_chunk_same_len_same_chunk_len
   {a: Type}
   (s1 s2: seq a)
-  (chunk_len: uint_size)
-  (chunk_num: uint_size)
+  (chunk_len: nat)
+  (chunk_num: nat)
   : Lemma
     (requires (LSeq.length s1 := LSeq.length s2 /\ chunk_len * chunk_num <= Seq.length s1))
     (ensures (seq_chunk_len s1 chunk_len chunk_lseq. Admitted. *)
 
-(* Definition seq_get_chunk
-  {a: Type}
-  (s: seq a)
-  (chunk_len: uint_size)
-  (chunk_num: uint_size)
-  : Pure (uint_size & seq a)
-    (requires (chunk_len * chunk_num <= Seq.length s))
-    (ensures (fun (out_len, chunk) ->
-      out_len := seq_chunk_len s chunk_len chunk_num /\ LSeq.length chunk := out_len
-    ))
- . :=
-  let idx_start := chunk_len * chunk_num in
-  let out_len := seq_chunk_len s chunk_len chunk_num in
-  (out_len, LSeq.slice #a #(Seq.length s)
-    s idx_start (idx_start + seq_chunk_len s chunk_len chunk_num)) *)
-
-(* Definition seq_set_chunk
-  {a: Type}
-  {len : uint_size} (* change to nseq but update_sub missing for nseq *)
-  (s: lseq a len)
-  (chunk_len: uint_size)
-  (chunk_num: uint_size)
-  (chunk: seq a )
-    : Pure (lseq a len)
-      (requires (
-        chunk_len * chunk_num <= Seq.length s /\
-        LSeq.length chunk := seq_chunk_len s chunk_len chunk_num
-      ))
-      (ensures (fun out -> True))
-  :=
- let idx_start := chunk_len * chunk_num in
- let out_len := seq_chunk_len s chunk_len chunk_num in
-  LSeq.update_sub s idx_start out_len chunk *)
-
-(**** Numeric operations *)
-
-Definition array_xor
-  {a: Type}
-  {len: uint_size}
-  (xor: a -> a -> a)
-  (s1: lseq a len)
-  (s2 : lseq a len)
-    : lseq a len
-  . Admitted.
-  (* :=
-  let out := s1 in
-  foldi 0 len (fun i out =>
-    array_upd out i (xor (array_index s1 i) (array_index s2 i))
-  ) out. *)
-
-Definition array_eq
-  {a: Type}
-  {len: uint_size}
-  (eq: a -> a -> bool)
-  (s1: lseq a len)
-  (s2 : lseq a len)
-    : bool
-  . Admitted.
-  (* :=
-  let out := true in
-  foldi 0 len (fun i out =>
-    andb out (eq (array_index s1 i) (array_index s2 i))
-  ) out. *)
-
-(* 
-Definition array_from_seq
-  {a: Type}
-  (out_len:uint_size)
-  (input: seq a{Seq.length input := out_len})
-    : lseq A out_len
-  := input. Admitted.
-
-Definition array_from_slice
-  {a: Type}
-  (default_value: a)
-  (out_len: uint_size)
-  (input: seq a)
-  (start: uint_size)
-  (slice_len: uint_size{start + slice_len <= LSeq.length input /\ slice_len <= out_len})
-    : lseq A out_len
-  :=
-  let out := LSeq.create out_len default_value in
-  LSeq.update_sub out 0 slice_len (LSeq.slice #a #(Seq.length input) input start (start + slice_len)). Admitted.
-
-Definition array_slice
-  {a: Type}
-  (input: seq a)
-  (start: uint_size)
-  (slice_len: uint_size{start + slice_len <= LSeq.length input})
-    : lseq A slice_len
-  :=
-  Seq.slice input start (start + slice_len).
-
-Definition array_from_slice_range
-  {a: Type}
-  (default_value: a)
-  (out_len: uint_size)
-  (input: seq a)
-  (start_fin: (uint_size & uint_size){
-     fst start_fin >= 0 /\ snd start_fin <= LSeq.length input /\ snd start_fin >= fst start_fin /\
-     snd start_fin - fst start_fin <= out_len
-   })
-    : lseq A out_len
- :=
-  let out := array_new_ default_value out_len in
-  let (start, fin) := start_fin in
-  LSeq.update_sub out 0 (fin - start) (Seq.slice input start fin).
-
-Definition array_slice_range
-  {a: Type}
-  {len : uint_size}
-  (input: lseq A len)
-  (start_fin:(uint_size & uint_size){
-    fst start_fin >= 0 /\ snd start_fin <= len /\ snd start_fin >= fst start_fin
-  })
-    : lseq A (snd start_fin - fst start_fin)uint_size
-  :=
-  let (start, fin) := start_fin in
-  LSeq.slice input start fin.
-
-Definition array_update_start
-  {a: Type}
-  {len: uint_size}
-  (s: lseq A len)
-  (start_s: seq a{Seq.length start_s <= len})
-    : lseq A len
-  :=
-  LSeq.update_sub s 0 (Seq.length start_s) start_s.
-
-Definition array_len  {a: Type} {len: uint_size} (s: lseq A len) := len
-
-(**** Seq manipulation *).
-
-Definition seq_slice
-  {a: Type}
-  (s: seq a)
-  (start: uint_size)
-  (len: uint_size{start + len <= LSeq.length s})
-    : lseq A len
-  :=
-  LSeq.slice #a #(Seq.length s) s start (start + len).
-
-Definition seq_update
-  {a: Type}
-  (s: seq a)
-  (start: uint_size)
-  (input: seq a{start + LSeq.length input <= LSeq.length s})
-    : nseq a (LSeq.length s)
-  :=
-  LSeq.update_sub #a #(LSeq.length s) s start (LSeq.length input) input.
-
-Definition seq_concat
-  {a: Type}
-  (s1 :seq a)
-  (s2: seq a{range (LSeq.length s1 + LSeq.length s2) U32})
-  : lseq A (LSeq.length s1 + LSeq.length s2)
-  :=
-  LSeq.concat #a #(LSeq.length s1) #(LSeq.length s2) s1 s2
-
-
-(**** Chunking *).
-
-Definition seq_num_chunks {a: Type} (s: seq a) (chunk_len: uint_size{chunk_len > 0}) : uint_size :=
-  (Seq.length s + chunk_len - 1) / chunk_len.
-
-Definition seq_chunk_len
-  {a: Type}
-  (s: seq a)
-  (chunk_len: uint_size)
-  (chunk_num: uint_size{chunk_len * chunk_num <= Seq.length s})
-    : Tot (out_len:uint_size{out_len <= chunk_len})
- . :=
-  Definition idx_start := chunk_len * chunk_num in
-  if idx_start + chunk_len > Seq.length s then
-    Seq.length s - idx_start
-  else
-    chunk_len.
-
-Definition seq_chunk_same_len_same_chunk_len
-  {a: Type}
-  (s1 s2: seq a)
-  (chunk_len: uint_size)
-  (chunk_num: uint_size)
-  : Lemma
-    (requires (LSeq.length s1 := LSeq.length s2 /\ chunk_len * chunk_num <= Seq.length s1))
-    (ensures (seq_chunk_len s1 chunk_len chunk_lseq.
-
 Definition seq_get_chunk
   {a: Type}
   (s: seq a)
-  (chunk_len: uint_size)
-  (chunk_num: uint_size)
-  : Pure (uint_size & seq a)
-    (requires (chunk_len * chunk_num <= Seq.length s))
-    (ensures (fun (out_len, chunk) ->
+  (chunk_len: nat)
+  (chunk_num: nat)
+  : (uint_size * seq a)
+    (* (requires (chunk_len * chunk_num <= Seq.length s))
+    (ensures (fun '(out_len, chunk) =>
       out_len := seq_chunk_len s chunk_len chunk_num /\ LSeq.length chunk := out_len
-    ))
- . :=
-  Definition idx_start := chunk_len * chunk_num in
-  Definition out_len := seq_chunk_len s chunk_len chunk_num in
-  (out_len, LSeq.slice #a #(Seq.length s)
-    s idx_start (idx_start + seq_chunk_len s chunk_len chunk_num))
+    )) *)
+ :=
+  let idx_start := chunk_len * chunk_num in
+  let out_len := seq_chunk_len s chunk_len chunk_num in
+  (usize out_len, slice
+    s idx_start (idx_start + seq_chunk_len s chunk_len chunk_num)).
 
 Definition seq_set_chunk
   {a: Type}
-  {len : uint_size} (* change to nseq but update_sub missing for nseq *)
-  (s: lseq A len)
-  (chunk_len: uint_size)
-  (chunk_num: uint_size)
+  {len : nat}
+  (s: nseq a len)
+  (chunk_len: nat)
+  (chunk_num: nat)
   (chunk: seq a )
-    : Pure (lseq A len)
-      (requires (
-        chunk_len * chunk_num <= Seq.length s /\
-        LSeq.length chunk := seq_chunk_len s chunk_len chunk_num
-      ))
-      (ensures (fun out -> True))
+    : nseq a len
   :=
-  Definition idx_start := chunk_len * chunk_num in
-  Definition out_len := seq_chunk_len s chunk_len chunk_num in
-  LSeq.update_sub s idx_start out_len chunk
+ let idx_start := chunk_len * chunk_num in
+ let out_len := seq_chunk_len (Vector.to_list s) chunk_len chunk_num in
+  update_sub s idx_start out_len chunk.
 
 (**** Numeric operations *)
 
 Definition array_xor
   {a: Type}
-  {len: uint_size}
+ `{Default a}
+  {len: nat}
   (xor: a -> a -> a)
-  (s1: lseq A len)
-  (s2 : lseq A len)
-    : lseq A len
+  (s1: nseq a len)
+  (s2 : nseq a len)
+    : nseq a len
   :=
-  Definition out := s1 in
-  foldi 0 len (fun i out ->
-    array_upd out i (array_index s1 i `xor` array_index s2 i)
-  ) out
+  let out := s1 in
+  foldi (usize 0) (usize len) (fun i out =>
+    let i := from_uint_size i in
+    array_upd out i (xor (array_index s1 i) (array_index s2 i))
+  ) out.
+
+Infix "array_xor_.^" := (array_xor xor) (at level 33) : hacspec_scope.
+
 
 Definition array_eq
   {a: Type}
-  {len: uint_size}
+  {len: nat}
   (eq: a -> a -> bool)
-  (s1: lseq A len)
-  (s2 : lseq A len)
-    : bool
-  :=
-  Definition out := true in
-  foldi 0 len (fun i out ->
-    out && (array_index s1 i `eq` array_index s2 i)
-  ) out *)
-
+  (s1: nseq a len)
+  (s2 : nseq a len)
+    : bool := Vector.eqb _ eq s1 s2.
 
 (**** Integers to arrays *)
-Axiom uint32_to_le_bytes : uint32 -> lseq uint8 4.
-(* Definition uint32_to_le_bytes (x: uint32) : lseq uint8 4 :=
+Axiom uint32_to_le_bytes : int32 -> nseq int8 4.
+(* Definition uint32_to_le_bytes (x: uint32) : nseq uint8 4 :=
   LBSeq.uint_to_bytes_le x. *)
 
-Axiom uint32_to_be_bytes : uint32 -> lseq uint8 4.
-(* Definition uint32_to_be_bytes (x: uint32) : lseq uint8 4 :=
+Axiom uint32_to_be_bytes : int32 -> nseq int8 4.
+(* Definition uint32_to_be_bytes (x: uint32) : nseq uint8 4 :=
   LBSeq.uint_to_bytes_be x *)
 
-Axiom uint32_from_le_bytes : lseq uint8 4 -> uint32.
-(* Definition uint32_from_le_bytes (s: lseq uint8 4) : uint32 :=
+Axiom uint32_from_le_bytes : nseq int8 4 -> int32.
+(* Definition uint32_from_le_bytes (s: nseq uint8 4) : uint32 :=
   LBSeq.uint_from_bytes_le s *)
 
-Axiom uint32_from_be_bytes : lseq uint8 4 -> uint32.
-(* Definition uint32_from_be_bytes (s: lseq uint8 4) : uint32 :=
+Axiom uint32_from_be_bytes : nseq int8 4 -> int32.
+(* Definition uint32_from_be_bytes (s: nseq uint8 4) : uint32 :=
   LBSeq.uint_from_bytes_be s *)
 
-Axiom uint64_to_le_bytes : uint64 -> lseq uint8 8.
-(* Definition uint64_to_le_bytes (x: uint64) : lseq uint8 8 :=
+Axiom uint64_to_le_bytes : int64 -> nseq int8 8.
+(* Definition uint64_to_le_bytes (x: uint64) : nseq uint8 8 :=
   LBSeq.uint_to_bytes_le x *)
 
-Axiom uint64_to_be_bytes : uint64 -> lseq uint8 8.
-(* Definition uint64_to_be_bytes (x: uint64) : lseq uint8 8 :=
+Axiom uint64_to_be_bytes : int64 -> nseq int8 8.
+(* Definition uint64_to_be_bytes (x: uint64) : nseq uint8 8 :=
   LBSeq.uint_to_bytes_be x *)
 
-Axiom uint64_from_le_bytes : lseq uint8 8 -> uint64.
-(* Definition uint64_from_le_bytes (s: lseq uint8 8) : uint64 :=
+Axiom uint64_from_le_bytes : nseq int8 8 -> int64.
+(* Definition uint64_from_le_bytes (s: nseq uint8 8) : uint64 :=
   LBSeq.uint_from_bytes_le s *)
 
-Axiom uint64_from_be_bytes : lseq uint8 8 -> uint64.
-(* Definition uint64_from_be_bytes (s: lseq uint8 8) : uint64 :=
+Axiom uint64_from_be_bytes : nseq int8 8 -> int64.
+(* Definition uint64_from_be_bytes (s: nseq uint8 8) : uint64 :=
   LBSeq.uint_from_bytes_be s *)
 
-Axiom uint128_to_le_bytes : uint128 -> lseq uint8 16.
-(* Definition uint128_to_le_bytes (x: uint128) : lseq uint8 16 :=
+Axiom uint128_to_le_bytes : int128 -> nseq int8 16.
+(* Definition uint128_to_le_bytes (x: uint128) : nseq uint8 16 :=
   LBSeq.uint_to_bytes_le x *)
 
-Axiom uint128_to_be_bytes : uint128 -> lseq uint8 16.
-(* Definition uint128_to_be_bytes (x: uint128) : lseq uint8 16 :=
+Axiom uint128_to_be_bytes : int128 -> nseq int8 16.
+(* Definition uint128_to_be_bytes (x: uint128) : nseq uint8 16 :=
   LBSeq.uint_to_bytes_be x *)
 
-Axiom uint128_from_le_bytes : lseq uint8 16 -> uint128.
-(* Definition uint128_from_le_bytes (input: lseq uint8 16) : uint128 :=
+Axiom uint128_from_le_bytes : nseq int8 16 -> int128.
+(* Definition uint128_from_le_bytes (input: nseq uint8 16) : uint128 :=
   LBSeq.uint_from_bytes_le input *)
 
-Axiom uint128_from_be_bytes : lseq uint8 16 -> uint128.
-(* Definition uint128_from_be_bytes (s: lseq uint8 16) : uint128 :=
+Axiom uint128_from_be_bytes : nseq int8 16 -> int128.
+(* Definition uint128_from_be_bytes (s: nseq uint8 16) : uint128 :=
   LBSeq.uint_from_bytes_be s *)
 
-Axiom u32_to_le_bytes : pub_uint32 -> lseq pub_uint8 4.
-(* Definition u32_to_le_bytes (x: pub_uint32) : lseq pub_uint8 4 :=
+Axiom u32_to_le_bytes : int32 -> nseq int8 4.
+(* Definition u32_to_le_bytes (x: pub_uint32) : nseq pub_uint8 4 :=
   LBSeq.uint_to_bytes_le x *)
 
-Axiom u32_to_be_bytes : pub_uint32 -> lseq pub_uint8 4.
-(* Definition u32_to_be_bytes (x: pub_uint32) : lseq pub_uint8 4 :=
+Axiom u32_to_be_bytes : int32 -> nseq int8 4.
+(* Definition u32_to_be_bytes (x: pub_uint32) : nseq pub_uint8 4 :=
   LBSeq.uint_to_bytes_be x *)
 
-Axiom u32_from_le_bytes : lseq pub_uint8 4 -> pub_uint32.
-(* Definition u32_from_le_bytes (s: lseq pub_uint8 4) : pub_uint32 :=
+Axiom u32_from_le_bytes : nseq int8 4 -> int32.
+(* Definition u32_from_le_bytes (s: nseq pub_uint8 4) : pub_uint32 :=
   LBSeq.uint_from_bytes_le s *)
 
-Axiom u32_from_be_bytes : lseq pub_uint8 4 -> pub_uint32.
-(* Definition u32_from_be_bytes (s: lseq pub_uint8 4) : pub_uint32 :=
+Axiom u32_from_be_bytes : nseq int8 4 -> int32.
+(* Definition u32_from_be_bytes (s: nseq pub_uint8 4) : pub_uint32 :=
   LBSeq.uint_from_bytes_be s *)
 
-Axiom u64_to_le_bytes : pub_uint64 -> lseq pub_uint8 8.
-(* Definition u64_to_le_bytes (x: pub_uint64) : lseq pub_uint8 8 :=
+Axiom u64_to_le_bytes : int64 -> nseq int8 8.
+(* Definition u64_to_le_bytes (x: int64) : nseq int8 8 :=
   LBSeq.uint_to_bytes_le x *)
 
-Axiom u64_to_be_bytes : pub_uint64 -> lseq pub_uint8 8.
-(* Definition u64_to_be_bytes (x: pub_uint64) : lseq pub_uint8 8 :=
+Axiom u64_to_be_bytes : int64 -> nseq int8 8.
+(* Definition u64_to_be_bytes (x: int64) : nseq int8 8 :=
   LBSeq.uint_to_bytes_be x *)
 
-Axiom u64_from_le_bytes : lseq pub_uint8 8 -> pub_uint64.
-(* Definition u64_from_le_bytes (s: lseq pub_uint8 8) : pub_uint64 :=
+Axiom u64_from_le_bytes : nseq int8 8 -> int64.
+(* Definition u64_from_le_bytes (s: nseq int8 8) : int64 :=
   LBSeq.uint_from_bytes_le s *)
 
-Axiom u64_from_be_bytes : lseq pub_uint8 8 -> pub_uint64.
-(* Definition u64_from_be_bytes (s: lseq pub_uint8 8) : pub_uint64 :=
+Axiom u64_from_be_bytes : nseq int8 8 -> int64.
+(* Definition u64_from_be_bytes (s: nseq int8 8) : int64 :=
   LBSeq.uint_from_bytes_be s *)
 
-Axiom u128_to_le_bytes : pub_uint128 -> lseq pub_uint8 16.
-(* Definition u128_to_le_bytes (x: pub_uint128) : lseq pub_uint8 16 :=
+Axiom u128_to_le_bytes : int128 -> nseq int8 16.
+(* Definition u128_to_le_bytes (x: int128) : nseq int8 16 :=
   LBSeq.uint_to_bytes_le x *)
 
-Axiom u128_to_be_bytes : pub_uint128 -> lseq pub_uint8 16.
-(* Definition u128_to_be_bytes (x: pub_uint128) : lseq pub_uint8 16 :=
+Axiom u128_to_be_bytes : int128 -> nseq int8 16.
+(* Definition u128_to_be_bytes (x: int128) : nseq int8 16 :=
   LBSeq.uint_to_bytes_be x *)
 
-Axiom u128_from_le_bytes : lseq pub_uint8 16 -> pub_uint128.
-(* Definition u128_from_le_bytes (input: lseq pub_uint8 16) : pub_uint128 :=
+Axiom u128_from_le_bytes : nseq int8 16 -> int128.
+(* Definition u128_from_le_bytes (input: nseq int8 16) : int128 :=
   LBSeq.uint_from_bytes_le input *)
 
-Axiom u128_from_be_bytes : lseq pub_uint8 16 -> pub_uint128.
-(* Definition u128_from_be_bytes (s: lseq pub_uint8 16) : pub_uint128 :=
+Axiom u128_from_be_bytes : nseq int8 16 -> int128.
+(* Definition u128_from_be_bytes (s: nseq int8 16) : pub_uint128 :=
   LBSeq.uint_from_bytes_be s *)
 
 (*** Nats *)
 
-(* type representing nats less than n *)
-(* currently just discards the n *)
-Definition nat_mod (n : N) := N.
 
-(* Modular multiplicative inverse *)
-Axiom nat_inv : N -> N -> N. 
+Definition nat_mod (p : N) : Set := GZnZ.znz (Z.of_N p).
+(* Definition nat_mod (p : uint_size) := nat_mod (from_uint_size p). *)
 
-(* Definition nat_mod (n: nat) := {x : nat | x < n}. *)
+Definition nat_mod_zero {p : N} : nat_mod p := GZnZ.zero (Z.of_N p).
+Definition nat_mod_one {p : N} : nat_mod p := GZnZ.one (Z.of_N p).
+Definition nat_mod_two {p : N} : nat_mod p := GZnZ.mkznz (Z.of_N p) _ (GZnZ.modz (Z.of_N p) 2).
 
-(* 
-Definition nat_mod_add {n:nat} (a:nat_mod n) (b:nat_mod n) : nat_mod n.
+
+(* convenience coercions from nat_mod to Z and N *)
+Coercion Z.of_N : N >-> Z.
+
+Definition nat_mod_add {n : N} (a : nat_mod n) (b : nat_mod n) : nat_mod n := GZnZ.add n a b.
+   
+Infix "+%" := nat_mod_add (at level 33) : hacspec_scope.
+
+Definition nat_mod_mul {n : N} (a:nat_mod n) (b:nat_mod n) : nat_mod n := GZnZ.add n a b.
+Infix "*%" := nat_mod_mul (at level 33) : hacspec_scope.
+
+Definition nat_mod_sub {n : N} (a:nat_mod n) (b:nat_mod n) : nat_mod n := GZnZ.sub n a b.
+Infix "-%" := nat_mod_mul (at level 33) : hacspec_scope.
+
+Definition nat_mod_div {n : N} (a:nat_mod n) (b:nat_mod n) : nat_mod n := GZnZ.div n a b.
+Infix "/%" := nat_mod_mul (at level 33) : hacspec_scope.
+
+Definition nat_modeg {n : N} (a:nat_mod n) : nat_mod n := GZnZ.opp n a.
+
+Definition nat_mod_inv {n : N} (a:nat_mod n) : nat_mod n := GZnZ.inv n a.
+
+Definition nat_mod_exp {p : N} (a:nat_mod p) (n : uint_size) : nat_mod p :=
+  let n : nat := Z.to_nat (from_uint_size n) in 
+  let fix exp_ (e : nat_mod p) (n : nat) :=
+    match n with
+    | 0%nat => nat_mod_one
+    | S n => nat_mod_mul a (exp_ a n)
+    end in
+  exp_ a n.
+
+Close Scope nat_scope.
+Open Scope Z_scope.
+
+(* We assume x < m *)
+Definition nat_mod_from_secret_literal {m : N} (x:int128) : nat_mod m.
 Proof.
-  unfold nat_mod. destruct a. destruct b.
-  apply (exist _ (x + x0 mod n)).
-   *)
-Definition nat_mod_add {n:N} (a : nat_mod n) (b : nat_mod n) : nat_mod n. Admitted.
+  unfold nat_mod.
+  (* since we assume x < m, it will be true that (unsigned x) = (unsigned x) mod m  *)
+  remember ((unsigned x) mod m) as zmodm.
+  apply (GZnZ.mkznz m zmodm).
+  rewrite Heqzmodm.
+  rewrite Zmod_mod.
+  reflexivity.
+Defined.
 
-Infix "+" := nat_mod_add : hacspec_scope.
+Definition nat_mod_from_literal (m : N) (x:int128) : nat_mod m := nat_mod_from_secret_literal x.
 
+Axiom nat_mod_to_public_byte_seq_le : forall (n : N) (len : uint_size), nat_mod n -> nseq int8 (from_uint_size len).
 
-Definition nat_mod_mul {n:N} (a:nat_mod n) (b:nat_mod n) : nat_mod n :=
-  (a * b) mod n.
+Definition nat_mod_bit {n : N} (a : nat_mod n) (i : uint_size) :=
+  Z.testbit (GZnZ.val n a) (from_uint_size i).
 
-Infix "*" := nat_mod_mul : hacspec_scope.
-
-Axiom uint128_to_N : uint128 -> N.
-
-Definition nat_from_secret_literal (m:N) (x:uint128) : nat_mod m :=
-  uint128_to_N x.
-
-Axiom pub_uint128_to_N : pub_uint128 -> N.
-
-Definition nat_from_literal (m:N) (x:pub_uint128) : nat_mod m :=
-  pub_uint128_to_N x.
 
 (*   
-Definition nat_to_public_byte_seq_le (n: pos)  (len: uint_size) (x: nat_mod n) : lseq pub_uint8 len =
+Definition nat_mod_to_public_byte_seq_le (n: pos)  (len: uint_size) (x: nat_mod_mod n) : lseq pub_uint8 len =
   Definition n' := n % (pow2 (8 * len)) in
-  Lib.ByteSequence.nat_to_bytes_le len n'
+  Lib.ByteSequence.nat_mod_to_bytes_le len n'*)
 
-Definition nat_to_public_byte_seq_be (n: pos)  (len: uint_size) (x: nat_mod n) : lseq pub_uint8 len =
+Axiom nat_mod_to_public_byte_seq_be : forall (n : N) (len : uint_size), nat_mod n -> nseq int8 (from_uint_size len).
+(* Definition nat_to_public_byte_seq_be (n: pos)  (len: uint_size) (x: nat_mod n) : lseq pub_uint8 len =
   Definition n' := n % (pow2 (8 * len)) in
   Lib.ByteSequence.nat_to_bytes_be len n' *)
 
+Axiom array_to_le_bytes : forall {A l}, nseq A l -> nseq int64 l.
+Axiom nat_mod_from_byte_seq_le : forall  {A l n}, nseq A l -> nat_mod n.  
+Axiom most_significant_bit : forall {m}, nat_mod m -> uint_size -> uint_size.
 
-Definition nat_pow2 (m : N) (x : N) : nat_mod m := pow2 x.
+
+(* We assume 2^x < m *)
+Definition nat_mod_pow2 (m : N) (x : N) : nat_mod m.
+Proof.
+  remember (Z.pow 2 x mod m) as y.
+  apply (GZnZ.mkznz m y).
+  rewrite Heqy.
+  rewrite Zmod_mod.
+  reflexivity.
+Defined.
+
+Section Coercions.
+
+  (* Integer coercions *)
+  (* We have nat >-> N >-> Z >-> int/int32 *)
+  Global Coercion repr : Z >-> int.
+  
+  Definition Z_to_int `{WORDSIZE} (n : Z) : int := repr n.
+  Global Coercion  Z_to_int : Z >-> int.
+
+  Definition Z_to_uint_size (n : Z) : uint_size := repr n.
+  Global Coercion Z_to_uint_size : Z >-> uint_size.
+  Definition Z_to_int_size (n : Z) : int_size := repr n.
+  Global Coercion Z_to_int_size : Z >-> int_size.
+
+  Definition N_to_int `{WORDSIZE} (n : N) : int := repr (Z.of_N n).
+  Global Coercion N.of_nat : nat >-> N.
+  Global Coercion N_to_int : N >-> int.
+  Definition N_to_uint_size (n : N) : uint_size := repr n.
+  Global Coercion N_to_uint_size : N >-> uint_size.
+  Definition nat_to_int `{WORDSIZE} (n : nat) := repr (Z.of_nat n).
+  Global Coercion nat_to_int : nat >-> int.  
+  Definition uint_size_to_nat (n : uint_size) : nat := from_uint_size n.
+  Global Coercion uint_size_to_nat : uint_size >-> nat.
+
+  Global Coercion GZnZ.val : GZnZ.znz >-> Z.
+
+  (* coercions into nat_mod *)
+  Definition Z_in_nat_mod {m : N} (x:Z) : nat_mod m.
+  Proof.
+    unfold nat_mod.
+    remember ((x) mod m) as zmodm.
+    apply (GZnZ.mkznz m zmodm).
+    rewrite Heqzmodm.
+    rewrite Zmod_mod.
+    reflexivity.
+  Defined.
+  Global Coercion Z_in_nat_mod : Z >-> nat_mod. 
+
+  Definition int_in_nat_mod {m : N} `{WORDSIZE} (x:int) : nat_mod m.
+  Proof.
+    unfold nat_mod.
+    (* since we assume x < m, it will be true that (unsigned x) = (unsigned x) mod m  *)
+    remember ((unsigned x) mod m) as zmodm.
+    apply (GZnZ.mkznz m zmodm).
+    rewrite Heqzmodm.
+    rewrite Zmod_mod.
+    reflexivity.
+    Show Proof.
+  Defined.
+  Global Coercion int_in_nat_mod : int >-> nat_mod.
+   
+  Definition uint_size_in_nat_mod (n : uint_size) : nat_mod 16 := int_in_nat_mod n.
+  Coercion uint_size_in_nat_mod : uint_size >-> nat_mod.
+
+End Coercions.
+
+
+
+(* Comparisons, boolean equality, and notation *)
+
+Class EqDec (A : Type) :=
+  { eqb : A -> A -> bool ;
+    eqb_leibniz : forall x y, eqb x y = true -> x = y }.
+
+Infix "=.?" := eqb (at level 40) : hacspec_scope.
+Infix "!=.?" := (fun a b => negb (eqb a b)) (at level 40) : hacspec_scope.
+
+Class Comparable (A : Type) := {
+  ltb : A -> A -> bool;
+  leb : A -> A -> bool;
+  gtb : A -> A -> bool;
+  geb : A -> A -> bool;
+}.
+Infix "<.?" := ltb (at level 42) : hacspec_scope.
+Infix "<=.?" := leb (at level 42) : hacspec_scope.
+Infix ">.?" := gtb (at level 42) : hacspec_scope.
+Infix ">=.?" := geb (at level 42) : hacspec_scope.
+
+Global Program Instance nat_eqdec : EqDec nat := {
+  eqb := Nat.eqb;
+  eqb_leibniz :=  fun a b => proj1 (Nat.eqb_eq a b) ;
+}.
+
+Global Instance nat_comparable : Comparable nat := {
+  ltb := Nat.ltb;
+  leb := Nat.leb;
+  gtb a b := Nat.ltb b a; 
+  geb a b := Nat.leb b a;
+}.
+
+Global Instance N_eqdec : EqDec N := {
+  eqb := N.eqb;
+  eqb_leibniz :=  fun a b => proj1 (N.eqb_eq a b) ;
+}.
+
+Global Instance N_comparable : Comparable N := {
+  ltb := N.ltb;
+  leb := N.leb;
+  gtb a b := N.ltb b a; 
+  geb a b := N.leb b a;
+}.
+
+Global Instance Z_eqdec : EqDec Z := {
+  eqb := Z.eqb;
+  eqb_leibniz :=  fun a b => proj1 (Z.eqb_eq a b) ;
+}.
+
+Global Instance Z_comparable : Comparable Z := {
+  ltb := Z.ltb;
+  leb := Z.leb;
+  gtb a b := Z.ltb b a; 
+  geb a b := Z.leb b a;
+}.
+
+Lemma int_eqb_eq : forall {WS : WORDSIZE} (a b : int), eq a b = true <-> a = b.
+Proof.
+  intros. split.
+  - apply same_if_eq.
+  - intros. rewrite H. apply eq_true.
+Qed.
+
+Global Instance int_eqdec `{WORDSIZE}: EqDec int := {
+  eqb := eq;
+  eqb_leibniz :=  fun a b => proj1 (int_eqb_eq a b) ;
+}.
+
+Global Instance int_comparable `{WORDSIZE} : Comparable int := {
+  ltb := lt;
+  leb a b := if eq a b then true else lt a b ;
+  gtb a b := lt b a; 
+  geb a b := if eq a b then true else lt b a;
+}.
+
+Definition nat_mod_val (p : N) (a : nat_mod p) : Z := GZnZ.val p a.
+
+Axiom nat_mod_eqb_spec : forall {p} (a b : nat_mod p), Z.eqb (nat_mod_val p a) (nat_mod_val p b) = true -> a = b.
+
+Global Instance nat_mod_eqdec {p} : EqDec (nat_mod p) := {
+  eqb a b := Z.eqb (nat_mod_val p a) (nat_mod_val p b);
+  eqb_leibniz := nat_mod_eqb_spec;
+}.
+
+Global Instance nat_mod_comparable `{p : N} : Comparable (nat_mod p) := {
+  ltb a b := Z.ltb (nat_mod_val p a) (nat_mod_val p b);
+  leb a b := if Zeq_bool a b then true else Z.ltb (nat_mod_val p a) (nat_mod_val p b) ;
+  gtb a b := Z.ltb (nat_mod_val p b) (nat_mod_val p a); 
+  geb a b := if Zeq_bool b a then true else Z.ltb (nat_mod_val p b) (nat_mod_val p a) ;
+}.
+
+Global Instance bool_eqdec : EqDec bool := {
+  eqb := Bool.eqb;
+  eqb_leibniz := Bool.eqb_prop;
+}.
+
+Global Instance string_eqdec : EqDec String.string := {
+  eqb := String.eqb;
+  eqb_leibniz :=  fun a b => proj1 (String.eqb_eq a b) ;
+}.
+
+Require Import Sumbool.
+Open Scope list_scope.
+
+Fixpoint list_eqdec {A} `{EqDec A} (l1 l2 : list A) : bool :=
+  match l1, l2 with
+  | x::xs, y::ys => if eqb x y then list_eqdec xs ys else false
+  | [], [] => true
+  | _,_ => false
+  end.
+
+Lemma list_eqdec_sound : forall {A} `{EqDec A} (l1 l2 : list A), list_eqdec l1 l2 = true -> l1 = l2.
+Proof.
+  intros A H l1. induction l1; intros; induction l2; simpl in *; try reflexivity; try inversion H0.
+   (* inductive case *)
+  apply Field_theory.if_true in H0; destruct H0.
+  f_equal.
+  (* show heads are equal *)
+  - apply (eqb_leibniz a a0 H0).
+  (* show tails are equal using induction hypothesis *)
+  - apply IHl1. assumption. 
+Qed.
+
+
+Global Instance List_eqdec {A} `{EqDec A} : EqDec (list A) := {
+  eqb := list_eqdec; 
+  eqb_leibniz := list_eqdec_sound;
+}.
+Require Import Program.Equality.
+Lemma vector_eqb_sound : forall {A : Type} {n : nat} `{EqDec A} (v1 v2 : t A n), Vector.eqb _ eqb v1 v2 = true -> v1 = v2.
+Proof.
+  intros A n H v1. induction v1; intros; simpl in *; dependent destruction v2.
+  - reflexivity.
+  - f_equal; rewrite Bool.andb_true_iff in H0; destruct H0.
+    + apply eqb_leibniz. assumption.
+    + apply IHv1. assumption.
+Qed.
+
+Global Program Instance Vector_eqdec {A n} `{EqDec A}: EqDec (Vector.t A n) := {
+  eqb := Vector.eqb _ eqb; 
+  eqb_leibniz := vector_eqb_sound;
+}.
+
+Global Program Instance Dec_eq_prod (A B : Type) `{EqDec A} `{EqDec B} : EqDec (A * B) := {
+  eqb '(a0, b0) '(a1, b1) := andb (eqb a0 a1) (eqb b0 b1)
+}.
+Next Obligation.
+  symmetry in H1.
+  apply Bool.andb_true_eq in H1. destruct H1.
+  symmetry in H1. apply (eqb_leibniz a0 a) in H1.
+  symmetry in H2. apply (eqb_leibniz b0 b) in H2.
+  rewrite H1, H2. reflexivity.
+Defined.
+
+
+(* Axiom most_significant_bit : scalar -> uint_size -> uint_size. *)
+
+
+
+
+(* Require Import DecidableClass.
+Global Instance nat_mod_eq_dec {p : N} (a b : nat_mod p) : Decidable (a = b) := {
+  Decidable_witness := eqb a b;
+  Decidable_spec := eqb_spec a b;
+}.
+
+Global Instance nat_mod_eq_dec {p} (a b : nat_mod p) : Decidable (a = b) := {
+  Decidable_witness := eqb a b;
+  Decidable_spec := eqb_spec a b;
+}.
+
+
+Definition decide_eq {A : Type} (a b : A) `{Decidable (a = b)}  := decide (a = b).
+Infix "==?" := decide_eq (at level 40) : hacspec_scope.
+
+(* Comparable instances have decidable equality *)
+Instance Comparable_to_Decidable {A} `(Comparable A) {a b : A} : Decidable (a = b) := {
+  Decidable_witness := eqb a b;
+  Decidable_spec := eqb_spec a b;
+}.
+
+
+
+ *)
